tests/lean/apply_tac.lean
@@ -38,3 +38,31 @@ begin
   apply le_refl,
   apply le_refl
 end
+
+def f (a := 10) : ℕ := a + 1
+
+def bla : nat :=
+begin
+  apply f -- uses opt_param for solving goal
+end
+
+example : bla = 11 :=
+rfl
+
+open tactic
+
+lemma foo {a b c : nat} (h₁ : a = b) (h₂ : b = c . assumption) : a = c :=
+eq.trans h₁ h₂
+
+example (a b c : nat) (h₁ : a = b) (h₂ : b = c) : a = c :=
+begin
+  apply foo h₁ -- uses auto_param for solving goal
+end
+
+lemma my_div_self (a : nat) (h : a ≠ 0 . assumption) : a / a = 1 :=
+sorry
+
+example (a : nat) (h : a ≠ 0) : a / a = 1 :=
+begin
+  apply my_div_self -- uses auto_param for solving goal
+end
